@prefix : <http://data.hulib.helsinki.fi/attx/onto#> .
@prefix cc: <https://creativecommons.org/ns#> .
@prefix owl: <http://www.w3.org/2002/07/owl#> .
@prefix pwo: <http://purl.org/spar/pwo/> .
@prefix rdf: <http://www.w3.org/1999/02/22-rdf-syntax-ns#> .
@prefix xml: <http://www.w3.org/XML/1998/namespace> .
@prefix xsd: <http://www.w3.org/2001/XMLSchema#> .
@prefix prov: <http://www.w3.org/ns/prov#> .
@prefix rdfs: <http://www.w3.org/2000/01/rdf-schema#> .
@prefix dcterms: <http://purl.org/dc/terms/> .
@base <http://data.hulib.helsinki.fi/attx/onto#> .

<http://data.hulib.helsinki.fi/attx/onto#> rdf:type owl:Ontology ;
                                            owl:versionIRI <http://data.hulib.helsinki.fi/attx/onto#> ;
                                            rdfs:comment "This ontology is published by the ATTX project, part of the University of Helsinki Library."@en ;
                                            <http://purl.org/dc/elements/1.1/date> "2017-05-04" ;
                                            owl:versionInfo "ATTX Workflow ontology 1.1"@en ;
                                            rdfs:seeAlso "http://helsinki.fi/library"@en ;
                                            <http://purl.org/dc/elements/1.1/creator> "ATTX project team" ;
                                            rdfs:label "ATTX Workflow Ontology"@en ;
                                            <http://purl.org/dc/elements/1.1/rights> "This work is licensed under a Creative Commons Attribution 4.0 International License." ,
                                                                                     "This work is licensed under a Creative Commons Attribution 4.0 International License http://creativecommons.org/licenses/by/4.0/" .

#################################################################
#    Annotation properties
#################################################################

###  http://purl.org/dc/elements/1.1/creator
<http://purl.org/dc/elements/1.1/creator> rdf:type owl:AnnotationProperty .


###  http://purl.org/dc/elements/1.1/date
<http://purl.org/dc/elements/1.1/date> rdf:type owl:AnnotationProperty .


###  http://purl.org/dc/elements/1.1/rights
<http://purl.org/dc/elements/1.1/rights> rdf:type owl:AnnotationProperty .


###  http://www.w3.org/2000/01/rdf-schema#comment
rdfs:comment rdf:type owl:AnnotationProperty .


###  http://www.w3.org/2004/02/skos/core#altLabel
<http://www.w3.org/2004/02/skos/core#altLabel> rdf:type owl:AnnotationProperty .


###  http://www.w3.org/2004/02/skos/core#prefLabel
<http://www.w3.org/2004/02/skos/core#prefLabel> rdf:type owl:AnnotationProperty .


#################################################################
#    Object Properties
#################################################################

###  http://creativecommons.org/ns#license
<http://creativecommons.org/ns#license> rdf:type owl:ObjectProperty ;
                                        rdfs:range <http://creativecommons.org/ns#License> ;
                                        rdfs:comment "Associated License for a specific dataset."@en .


###  http://data.hulib.helsinki.fi/attx/onto#hasAssociatedGraph
:hasAssociatedGraph rdf:type owl:ObjectProperty ;
                    rdfs:domain :Step ;
                    rdfs:range :Dataset ;
                    rdfs:comment "A Step can make use of a certain graph/dataset besides the input graph."@en ;
                    rdfs:label "hasAssociatedGraph"@en .


###  http://data.hulib.helsinki.fi/attx/onto#hasStrategyType
:hasStrategyType rdf:type owl:ObjectProperty ;
                 rdfs:comment "The current strategy if a derivate of a specific type of Linking Strategy."@en .


###  http://data.hulib.helsinki.fi/attx/onto#isDependentOn
:isDependentOn rdf:type owl:ObjectProperty ;
               rdfs:domain :Artifact ;
               rdfs:range :Artifact ;
               rdfs:comment "An artifact can be depenednt on other artifacts in order to perform an activity."@en ;
               rdfs:label "isDependentOn"@en .


###  http://data.hulib.helsinki.fi/attx/onto#usesArtifact
:usesArtifact rdf:type owl:ObjectProperty ;
              rdfs:subPropertyOf prov:used ;
              rdfs:range :Artifact ;
              rdfs:comment "An artifact can be used by any type of entity or resource in order to perform certain steps/activities."@en ;
              rdfs:label "usesArtifact"@en .


###  http://data.hulib.helsinki.fi/attx/onto#usesWorkflowExecution
:usesWorkflowExecution rdf:type owl:ObjectProperty ;
                       rdfs:subPropertyOf owl:topObjectProperty ;
                       rdfs:domain :Workflow ;
                       rdfs:range :WorkflowExecution ;
                       rdfs:comment "Specify the Workflow Execution associated with a current Workflow."@en ;
                       rdfs:label "usesWorkflowExecution"@en .


###  http://purl.org/spar/pwo/hasFirstStep
pwo:hasFirstStep rdf:type owl:ObjectProperty ;
                 rdfs:domain :Workflow ;
                 rdfs:range :Step ;
                 rdfs:comment "A workflow that starts with a particular step."@en ;
                 rdfs:label "has first step"@en .


###  http://purl.org/spar/pwo/hasNextStep
pwo:hasNextStep rdf:type owl:ObjectProperty ;
                rdfs:domain :Step ;
                rdfs:range :Step ;
                rdfs:comment "A property linking a step in a workflow with the step that directly follows it."@en ;
                rdfs:label "has next step"@en .


###  http://purl.org/spar/pwo/hasStep
pwo:hasStep rdf:type owl:ObjectProperty ;
            rdfs:domain :Workflow ;
            rdfs:range :Step ;
            rdfs:comment "The property linking a workflow to a component step."@en ;
            rdfs:label "has step"@en .


###  http://www.w3.org/ns/prov#agent
prov:agent rdf:type owl:ObjectProperty ;
           rdfs:range prov:Agent ;
           rdfs:comment "The prov:agent property references an prov:Agent which influenced a resource. This property applies to an prov:AgentInfluence, which is given by a subproperty of prov:qualifiedInfluence from the influenced prov:Entity, prov:Activity or prov:Agent."@en ;
           rdfs:label "agent"@en .


###  http://www.w3.org/ns/prov#generated
prov:generated rdf:type owl:ObjectProperty ;
               rdfs:domain prov:Activity ;
               rdfs:comment "Generation is the completion of production of a new entity by an activity. This entity did not exist before generation and becomes available for usage after this generation."@en ;
               rdfs:label "generated"@en .


###  http://www.w3.org/ns/prov#hadDerivation
prov:hadDerivation rdf:type owl:ObjectProperty ;
                   owl:inverseOf prov:wasDerivedFrom ;
                   rdfs:comment "Inverse of wasDerivedFrom property"@en ;
                   rdfs:label "hadDerivation"@en .


###  http://www.w3.org/ns/prov#hadPlan
prov:hadPlan rdf:type owl:ObjectProperty ;
             rdfs:domain prov:Association ;
             rdfs:range prov:Plan ;
             rdfs:comment "A plan is an entity that represents a set of actions or steps intended by one or more agents to achieve some goals."@en ;
             rdfs:label "hadPlan"@en .


###  http://www.w3.org/ns/prov#qualifiedAssociation
prov:qualifiedAssociation rdf:type owl:ObjectProperty ;
                          rdfs:comment "An activity association is an assignment of responsibility to an agent for an activity, indicating that the agent had a role in the activity. It further allows for a plan to be specified, which is the plan intended by the agent to achieve some goals in the context of this activity."@en ;
                          rdfs:label "qualifiedAssociation"@en .


###  http://www.w3.org/ns/prov#used
prov:used rdf:type owl:ObjectProperty ;
          rdfs:domain prov:Activity ;
          rdfs:comment "Usage is the beginning of utilizing an entity by an activity. Before usage, the activity had not begun to utilize this entity and could not have been affected by the entity."@en ;
          rdfs:label "used"@en .


###  http://www.w3.org/ns/prov#wasAssociatedWith
prov:wasAssociatedWith rdf:type owl:ObjectProperty ;
                       rdfs:domain prov:Activity ;
                       rdfs:range prov:Agent ;
                       rdfs:comment "An activity association is an assignment of responsibility to an agent for an activity, indicating that the agent had a role in the activity. It further allows for a plan to be specified, which is the plan intended by the agent to achieve some goals in the context of this activity."@en ;
                       rdfs:label "wasAssociatedWith"@en .


###  http://www.w3.org/ns/prov#wasDerivedFrom
prov:wasDerivedFrom rdf:type owl:ObjectProperty ;
                    rdfs:comment "A derivation is a transformation of an entity into another, an update of an entity resulting in a new one, or the construction of a new entity based on a pre-existing entity."@en ;
                    rdfs:label "wasDerivedFrom"@en .


#################################################################
#    Data properties
#################################################################

###  http://data.hulib.helsinki.fi/attx/onto#hasStepConfig
:hasStepConfig rdf:type owl:DatatypeProperty ;
               rdfs:comment "A Step can have different configurations associated to with which specifies the Workflow how to perform the given step."@en ;
               rdfs:label "hasStepConfig"@en .


###  http://www.w3.org/ns/prov#endedAtTime
prov:endedAtTime rdf:type owl:DatatypeProperty ;
                 rdfs:domain prov:Activity ;
                 rdfs:range xsd:dateTime ;
                 rdfs:comment "End is when an activity is deemed to have been ended by an entity, known as trigger. The activity no longer exists after its end. Any usage, generation, or invalidation involving an activity precedes the activity's end. An end may refer to a trigger entity that terminated the activity, or to an activity, known as ender that generated the trigger."@en ;
                 rdfs:label "endedAtTime"@en .


###  http://www.w3.org/ns/prov#startedAtTime
prov:startedAtTime rdf:type owl:DatatypeProperty ;
                   rdfs:domain prov:Activity ;
                   rdfs:range xsd:dateTime ;
                   rdfs:comment "Start is when an activity is deemed to have been started by an entity, known as trigger. The activity did not exist before its start. Any usage, generation, or invalidation involving an activity follows the activity's start. A start may refer to a trigger entity that set off the activity, or to an activity, known as starter, that generated the trigger."@en ;
                   rdfs:label "startedAtTime"@en .


#################################################################
#    Classes
#################################################################

###  http://creativecommons.org/ns#License
<http://creativecommons.org/ns#License> rdf:type owl:Class ;
                                        rdfs:comment "A set of requests/permissions to users of a Work, e.g. a copyright license, the public domain, information for distributors"@en ;
                                        rdfs:label "License"@en .


###  http://data.hulib.helsinki.fi/attx/onto#AcquisitionWorkflow
:AcquisitionWorkflow rdf:type owl:Class ;
                     rdfs:subClassOf :Workflow ;
                     rdfs:comment "A sequence of dependent steps, with the main goal of acquiring/importing/accessing information from a specific source."@en ;
                     rdfs:label "Acquisition Workflow"@en .


###  http://data.hulib.helsinki.fi/attx/onto#Artifact
:Artifact rdf:type owl:Class ;
          rdfs:comment "An artifact is a type of mutable or imutable resource used in a specific workflow. Examples: Web Service, source code or any other type of software component and not only."@en ;
          rdfs:label "Artifact"@en .


###  http://data.hulib.helsinki.fi/attx/onto#Dataset
:Dataset rdf:type owl:Class ;
         rdfs:comment "A specific resource which represents a Dataset used in an workflow."@en ;
         rdfs:label "Dataset"@en .


###  http://data.hulib.helsinki.fi/attx/onto#DisseminationWorkflow
:DisseminationWorkflow rdf:type owl:Class ;
                       rdfs:subClassOf :Workflow ;
                       rdfs:comment "A sequence of dependent steps, representing a series of activities that make it possible to publish and distribute information (e.g. via an API)."@en ;
                       rdfs:label "Dissemination Workflow"@en .


###  http://data.hulib.helsinki.fi/attx/onto#EnrichmentWorkflow
:EnrichmentWorkflow rdf:type owl:Class ;
                    rdfs:subClassOf :Workflow ;
                    rdfs:comment "A sequence steps that have the main purpose of enriching information from a specific Dataset. The act of enriching can be performed by a specific artifact and can vary from simple linkage and/or adding new properties to complex inferecing."@en ;
                    rdfs:label "Enrichment Workflow"@en .


###  http://data.hulib.helsinki.fi/attx/onto#InputStep
:InputStep rdf:type owl:Class ;
           rdfs:subClassOf :Step ;
           rdfs:comment "A specif action/type of activity performed in an Workflow, that has associated an input (always a Data Graph) at the beginning of the Workflow."@en ;
           rdfs:label "Input Step"@en .


###  http://data.hulib.helsinki.fi/attx/onto#LinkingStrategy
:LinkingStrategy rdf:type owl:Class ;
                 rdfs:comment "A Linking Strategy represents an operation or a set of operations with different parameters that has the purpose to connection two or more datasets. There can be multiple types of strategies (e.g. IDs strategy, NER, etc.), each type of strategy having multiple and distinct types of parameters (e.g. for SPARQL we can add parameters for the type of skos predicate to be used; for NER we can add multiple languages or training sets etc.)."@en ;
                 rdfs:label "Linking Strategy"@en .


###  http://data.hulib.helsinki.fi/attx/onto#MetadataStep
:MetadataStep rdf:type owl:Class ;
              rdfs:subClassOf :Step ;
              rdfs:comment "A specif action/type of activity performed in an Workflow, that registeres Metadata specific information about the current Workflow. This Step can be performed imediately after the InputStep or at any other point in the Workflow but not after the OutputStep."@en ;
              rdfs:label "Metadata Step"@en .


###  http://data.hulib.helsinki.fi/attx/onto#OutputStep
:OutputStep rdf:type owl:Class ;
            rdfs:subClassOf :Step ;
            rdfs:comment "A specif action/type of activity performed in an Workflow, that has associated an output (always a Working Data Graph) at the end of the Workflow."@en ;
            rdfs:label "Output Step"@en .


###  http://data.hulib.helsinki.fi/attx/onto#Process
:Process rdf:type owl:Class ;
         rdfs:comment "Process refers to an activity or series of actions (steps) caused by Agents, performed via a Worfklow and resulting in new Datasets."@en ;
         rdfs:label "Process"@en .


###  http://data.hulib.helsinki.fi/attx/onto#Step
:Step rdf:type owl:Class ;
      rdfs:subClassOf prov:Activity ;
      rdfs:comment "A specif action/type of activity performed in an Workflow, that may have associated a start time and an end time, and may be associated with one or more Artifacts."@en ;
      rdfs:label "Step"@en .


###  http://data.hulib.helsinki.fi/attx/onto#Workflow
:Workflow rdf:type owl:Class ;
          rdfs:subClassOf prov:Plan ;
          rdfs:comment "A sequence of dependent steps, representing a series of activities that make use of certain Artifacts and Datasets. A workflow is performed as part of a specific Plan and has associated a WorkflowExecution activity."@en ;
          rdfs:label "Workflow"@en .


###  http://data.hulib.helsinki.fi/attx/onto#WorkflowExecution
:WorkflowExecution rdf:type owl:Class ;
                   rdfs:subClassOf prov:Activity ;
                   rdfs:comment "A workflow execution represents the execution of a Workflow and is itself an Activity. The execution process can also describe the specific artifacts used to acomplish the Workflow, the Dataset and Agent described in the proces template."@en ;
                   rdfs:label "Workflow Execution"@en .


###  http://www.w3.org/ns/prov#Activity
prov:Activity rdf:type owl:Class ;
              rdfs:comment "An activity is something that occurs over a period of time and acts upon or with entities; it may include consuming, processing, transforming, modifying, relocating, using, or generating entities."@en ;
              rdfs:label "Activity"@en .


###  http://www.w3.org/ns/prov#Agent
prov:Agent rdf:type owl:Class ;
           rdfs:comment "An agent is something that bears some form of responsibility for an activity taking place, for the existence of an entity, or for another agent's activity."@en ;
           rdfs:label "Agent"@en .


###  http://www.w3.org/ns/prov#Association
prov:Association rdf:type owl:Class ;
                 rdfs:comment "An activity association is an assignment of responsibility to an agent for an activity, indicating that the agent had a role in the activity. It further allows for a plan to be specified, which is the plan intended by the agent to achieve some goals in the context of this activity."@en ;
                 rdfs:label "Association"@en .


###  http://www.w3.org/ns/prov#Plan
prov:Plan rdf:type owl:Class ;
          rdfs:comment "A plan is an entity that represents a set of actions or steps intended by one or more agents to achieve some goals."@en ,
                       "There exist no prescriptive requirement on the nature of plans, their representation, the actions or steps they consist of, or their intended goals. Since plans may evolve over time, it may become necessary to track their provenance, so plans themselves are entities. Representing the plan explicitly in the provenance can be useful for various tasks: for example, to validate the execution as represented in the provenance record, to manage expectation failures, or to provide explanations."@en ;
          rdfs:label "Plan"@en .


#################################################################
#    Individuals
#################################################################

###  http://data.hulib.helsinki.fi/attx/onto#CC0
:CC0 rdf:type owl:NamedIndividual ,
              <http://creativecommons.org/ns#License> ;
     rdfs:comment """CC0
“No Rights Reserved”""" ;
     rdfs:label "CreativeCommons 0" .


###  http://data.hulib.helsinki.fi/attx/onto#Unknown
:Unknown rdf:type owl:NamedIndividual ,
                  <http://creativecommons.org/ns#License> ;
         rdfs:comment "An Unknown license type, this means the license might contain copyrighted work."@en ;
         rdfs:label "Unknown"@en .


###  Generated by the OWL API (version 4.2.8.20170104-2310) https://github.com/owlcs/owlapi
